Simpler implementation of ARexp.

reals/faster/ARexp.v
@@ -11,9 +11,9 @@ Section ARexp.
 Context `{AppRationals AQ}.
 
 Section exp_small_neg.
-Context {a : AQ} (Pa : -(1) ≤ 'a ≤ 0).
+Context {a : AQ} (Pa : -1 ≤ a ≤ 0).
 
-Lemma ARexpSequence : DivisionStream (expSequence (- 'a)) (powers (-a)) factorials.
+Lemma ARexpSequence : DivisionStream (expSequence (-'a)) (powers (-a)) factorials.
 Proof.
   apply DivisionStream_Str_nth.
   intros n.
@@ -27,10 +27,17 @@ Proof.
   now rewrite preserves_factorials.
 Qed.
 
-Definition AQexp_small_neg : AR := ARInfAltSum ARexpSequence 
-  (dnn:=expSequence_dnn (Qle_ZO_flip Pa)) (zl:=expSequence_zl (Qle_ZO_flip Pa)).
+Definition AQexp_small_neg_prf : -1 ≤ 'a ≤ 0.
+Proof.
+  split.
+   now apply rings.preserves_ge_opp1.
+  now apply semirings.preserves_nonpos.
+Qed.
 
-Lemma ARexp_small_neg_correct : ARtoCR AQexp_small_neg = rational_exp ('a).
+Definition AQexp_small_neg : AR := ARInfAltSum ARexpSequence 
+  (dnn:=expSequence_dnn (Qle_ZO_flip AQexp_small_neg_prf)) (zl:=expSequence_zl (Qle_ZO_flip AQexp_small_neg_prf)).
+
+Lemma AQexp_small_neg_correct : ARtoCR AQexp_small_neg = rational_exp ('a).
 Proof.
   rewrite rational_exp_correct.
   rewrite <-rational_exp_small_neg_correct.
@@ -38,156 +45,145 @@ Proof.
 Qed.
 End exp_small_neg.
 
-Lemma AQexp_neg_bounded_prf `(Pa : inject_Z (-2^S n) ≤ 'a ≤ 0) : 
-  inject_Z (- 2^n) ≤ '(a ≪ -(1)) ≤ 0.
+Lemma AQexp_neg_bounded_prf `(Pa : -2^S n ≤ a ≤ 0) : 
+  -2^n ≤ a ≪ (-1) ≤ 0.
 Proof.
-  rewrite Zshift_opp_1.
-  now apply shrink_by_two.
-Qed. 
+  split.
+   apply (order_preserving_back (2 *.)).
+   rewrite <-shiftl_S, rings.plus_opp_r, shiftl_0.
+   now rewrite <-rings.distr_opp_mult_r.
+  apply (order_preserving_back (2 *.)).
+  rewrite <-shiftl_S, rings.plus_opp_r, shiftl_0.
+  now rewrite right_absorb.
+Qed.
 
-Fixpoint AQexp_neg_bounded {n : nat} {a : AQ} : inject_Z (-2^n) ≤ 'a ≤ 0 → AR :=
+Fixpoint AQexp_neg_bounded {n : nat} {a : AQ} : -2^n ≤ a ≤ 0 → AR :=
   match n with
   | O => AQexp_small_neg
   | S n' => λ Pa, ARpower_positive_bounded 2 1 (ARcompress (AQexp_neg_bounded (AQexp_neg_bounded_prf Pa)))
   end.
 
-Lemma AQexp_neg_bounded_correct {n : nat} {a : AQ} (Pa : inject_Z (-2^n) ≤ 'a ≤ 0) : 
+Lemma AQexp_neg_bounded_correct {n : nat} {a : AQ} (Pa : -2^n ≤ a ≤ 0) : 
   ARtoCR (AQexp_neg_bounded Pa) = rational_exp ('a).
 Proof.
   revert a Pa.
   induction n; intros a p.
-   apply ARexp_small_neg_correct.
+   apply AQexp_small_neg_correct.
   unfold AQexp_neg_bounded. fold (AQexp_neg_bounded (AQexp_neg_bounded_prf p)).
   rewrite ARtoCR_preserves_power_positive_bounded.
   rewrite ARcompress_correct.
   setoid_replace (AQposAsQpos 1) with (1#1)%Qpos by now rewrite AQposAsQpos_preserves_1.
   rewrite rational_exp_correct.
-  rewrite <-shrink_by_two_correct; [|easy].
-  rewrite <-rational_exp_correct.
-  rewrite IHn.
-  rewrite Zshift_opp_1. 
-  reflexivity.
+  rewrite <-shrink_by_two_correct.
+   rewrite <-rational_exp_correct.
+   rewrite IHn.
+   rewrite Zshift_opp_1. 
+   reflexivity.
+  now apply semirings.preserves_nonpos.
 Qed.
 
 Section exp_neg.
-Context {a : AQ} (Pa : 'a ≤ 0).
+Context {a : AQ} (Pa : a ≤ 0).
 
 Definition AQexp_neg_bound : nat := 
-  match decide_rel (≤) (-(1)) a with
+  match decide_rel (≤) (-1) a with
   | left _ => 0
   | right _ => Zabs_nat (Zsucc (Qdlog2 (-'a)))
   end.
 
-Lemma AQexp_neg_bound_correct :
-   inject_Z (-2 ^ AQexp_neg_bound) ≤ 'a ≤ 0.
+Lemma AQexp_neg_bound_correct : -2 ^ AQexp_neg_bound ≤ a ≤ 0.
 Proof.
   split; [|trivial].
   unfold AQexp_neg_bound.
   case (decide_rel (≤)); intros E1.
-   case (decide ('a = 0)); intros E2.
-    now rewrite E2.
-   transitivity (-(1):Q).
-    easy.
-   rewrite <-(rings.preserves_1 (f:=coerce : AQ → Q)).
-   rewrite <-rings.preserves_opp.
-   now apply (order_preserving _).
-  case (decide ('a = 0)); intros E2.
-   now rewrite E2.
-  rewrite inj_Zabs_nat.
-  assert (0 ≤ Qdlog2 (-'a)).
-   apply Qdlog2_nonneg. change (- -(1) ≤ -'a).
-   apply (proj1 (rings.flip_opp _ _)).
-   rewrite <-(rings.preserves_1 (f:=coerce : AQ → Q)).
-   rewrite <-rings.preserves_opp.
-   apply (order_preserving _).
-   now apply orders.precedes_flip.
-  rewrite Z.abs_eq.
-   rewrite <-(rings.opp_involutive ('a)) at 2.
-   posed_rewrite (rings.preserves_opp (f:=inject_Z)).
-   apply (proj1 (rings.flip_opp _ _)).
-   rewrite Qpower.Zpower_Qpower.
-    change (inject_Z 2) with (2:Q).
-    apply stdlib_rationals.Qlt_coincides.
-    apply Qdlog2_spec.
-    apply stdlib_rationals.Qlt_coincides.
-    apply rings.flip_neg_opp. now split.
-   now apply_simplified (semirings.nonneg_plus_compat (R:=Z)).
-  now apply Zle_le_succ.
+   easy.
+  apply orders.precedes_flip in E1.
+  apply (order_preserving_back (coerce : AQ → Q)).
+  rewrite rings.preserves_opp.
+  rewrite preserves_nat_pow.
+  rewrite rings.preserves_2.
+  rewrite <-(int_pow_nat_pow (f:=Z_of_nat)).
+  rewrite inj_Zabs_nat, Z.abs_eq.
+   apply rings.flip_opp.
+   rewrite rings.opp_involutive.
+   apply stdlib_rationals.Qlt_coincides.
+   apply Qdlog2_spec.
+   apply stdlib_rationals.Qlt_coincides.
+   apply rings.flip_neg_opp.
+   apply orders.sprecedes_trans_r with (-1).
+    now apply rings.preserves_le_opp1.
+   apply rings.flip_pos_opp. now apply semirings.sprecedes_0_1.
+  apply Zle_le_succ.
+  apply Qdlog2_nonneg. 
+  change (- -1 ≤ -'a).
+  apply rings.flip_opp.
+  now apply rings.preserves_le_opp1.
 Qed.
 
 (* We can also divide by any additional number of 2 powers. Doing this generally 
    improves the performance because the sequence diverges more quickly. *)
-Lemma AQexp_neg_bound_weaken (n : nat) :
-   inject_Z (-2 ^ Z_of_nat (n + AQexp_neg_bound)) ≤ 'a ≤ 0.
+Lemma AQexp_neg_bound_weaken (n : nat) : -2 ^ (n + AQexp_neg_bound) ≤ a ≤ 0.
 Proof.
   split; [|trivial].
-  transitivity (inject_Z (-2 ^ AQexp_neg_bound)).
-   apply (order_preserving _).
-   apply (proj1 (rings.flip_opp _ _)).
-   posed_rewrite (rings.preserves_plus (f:=Z_of_nat)).
-   rewrite Zpower_exp; auto with *.
+  transitivity (-2 ^ AQexp_neg_bound).
+   apply rings.flip_opp.
+   rewrite nat_pow_exp_plus.
    apply semirings.ge1_mult_compat_l.
-     now apply Z.pow_nonneg.
-    change (2 ^ 0 ≤ 2 ^ n)%Z.
-    apply Z.pow_le_mono_r; auto with *.
+     apply nat_pow_nonneg. apply _.
+    apply nat_pow_ge1. 
+     apply semirings.precedes_1_2.
+    apply naturals.naturals_nonneg.
    reflexivity.
   now apply AQexp_neg_bound_correct.
 Qed.
 
 Definition AQexp_neg : AR := AQexp_neg_bounded (AQexp_neg_bound_weaken 75).
 
-Lemma ARexp_neg_correct: ARtoCR AQexp_neg = rational_exp ('a).
+Lemma AQexp_neg_correct: ARtoCR AQexp_neg = rational_exp ('a).
 Proof. apply AQexp_neg_bounded_correct. Qed.
 
+(* We could use a number closer to 1/exp 1, for example 11 $ -5, but in practice this seems
+    to make it slower. *)
 Program Definition AQexp_inv_pos_bound : AQ₊ :=
-  let aQ := 'a in exist _ (('(1 : Z) ≪ -(2 : Z)) ^ Zabs_N (Zdiv (Qnum aQ) (Qden aQ))) _. (* 11 $ 5 *)
+  let b := 'a in ((1 ≪ -(2 : Z)) ^ Zabs_N (Zdiv (Qnum b) (Qden b)))↾_.
 Next Obligation.
   apply nat_pow_pos.
   apply (maps.strictly_order_preserving_back (coerce : AQ → Q)).
-  rewrite rings.preserves_0.
   rewrite aq_shift_correct.
-  apply semirings.pos_mult_scompat.
-   rewrite AQtoQ_ZtoAQ.
-   now apply stdlib_rationals.Qlt_coincides.
-  apply int_pow_pos.
-  now apply semirings.sprecedes_0_2.
+  rewrite rings.preserves_0, rings.preserves_1. 
+  split; easy.
 Qed.
 
 Lemma AQexp_inv_pos_bound_correct :
   '(AQposAsQpos AQexp_inv_pos_bound : Q) ≤ rational_exp ('a). 
 Proof.
   unfold AQexp_inv_pos_bound.
-  unfold AQposAsQpos, positive_semiring_elements.Pos_inject. simpl.
+  unfold AQposAsQpos. simpl. 
+  unfold coerce at 3. unfold positive_semiring_elements.Pos_inject. simpl.
   rewrite preserves_nat_pow.
   rewrite aq_shift_correct.
+  rewrite rings.preserves_1, left_identity.
   rewrite <-int_pow_nat_pow.
-  rewrite AQtoQ_ZtoAQ.
   rewrite Z_of_N_abs, Z.abs_neq.
    rewrite rational_exp_correct.
-   rewrite <-(rational_exp_neg_correct Pa).
+   rewrite <-(rational_exp_neg_correct (semirings.preserves_nonpos (f:=coerce : AQ → Q) a Pa)).
    pose proof (@rational_exp_neg_posH' (1%positive * 2 ^ -2)) as P.
    apply P. clear. unfold CRle. apply CRpos_nonNeg.
    CRsign.CR_solve_pos (1#1)%Qpos.
   apply Zdiv_le_upper_bound.
    auto with *.
   rewrite left_absorb.
-  now apply Qnum_nonpos.
+  apply Qnum_nonpos.
+  change ('a ≤ 0).
+  now apply semirings.preserves_nonpos.
 Qed.
 End exp_neg.
 
-Lemma AQexp_prf1 {a : AQ} (pA : 0 ≤ a) : '(-a) ≤ 0.
-Proof.
-  posed_rewrite <-(rings.preserves_0 (f:=coerce : AQ → Q)).
-  apply (order_preserving _).
-  now apply rings.flip_nonneg_opp.
-Qed.
+Lemma AQexp_prf1 {a : AQ} (pA : 0 ≤ a) : -a ≤ 0.
+Proof. now apply rings.flip_nonneg_opp. Qed.
 
-Lemma AQexp_prf2 {a : AQ} (pA : ¬0 ≤ a) : 'a ≤ 0.
-Proof.
-  posed_rewrite <-(rings.preserves_0 (f:=coerce : AQ → Q)).
-  apply (order_preserving _).
-  now apply orders.precedes_flip.
-Qed.
+Lemma AQexp_prf2 {a : AQ} (pA : ¬0 ≤ a) : a ≤ 0.
+Proof. now apply orders.precedes_flip. Qed.
 
 Definition AQexp (a : AQ) : AR := 
   match (decide_rel (≤) 0 a) with
@@ -195,39 +191,36 @@ Definition AQexp (a : AQ) : AR :=
   | right Pa => AQexp_neg (AQexp_prf2 Pa)
   end.
 
-Lemma ARexp_correct a : ARtoCR (AQexp a) = rational_exp ('a).
+Lemma AQexp_correct a : ARtoCR (AQexp a) = rational_exp ('a).
 Proof.
   unfold AQexp.
   case (decide_rel _); intros.
    rewrite ARtoCR_preserves_inv_pos.
-   rewrite ARexp_neg_correct.
+   rewrite AQexp_neg_correct.
    rewrite rings.preserves_opp.
    rewrite 2!rational_exp_correct.
    apply rational_exp_pos_correct.
-    posed_rewrite <-(rings.preserves_0 (f:=coerce : AQ → Q)).
-    now apply (order_preserving _).
+    now apply semirings.preserves_nonneg.
    rewrite <-rational_exp_correct.
    posed_rewrite <-(rings.preserves_opp (f:=coerce : AQ → Q)).
    apply AQexp_inv_pos_bound_correct.
-   posed_rewrite <-(rings.preserves_0 (f:=coerce : AQ → Q)).
-   apply (order_preserving _).
    now apply rings.flip_nonneg_opp.
-  apply ARexp_neg_correct.
+  apply AQexp_neg_correct.
 Qed.
 
 Local Obligation Tactic := idtac.
 Program Definition ARexp_bounded_uc (z : Z) := 
-  unary_complete_uc QPrelengthSpace coerce (λ x, AQexp (min ('z : AQ) x)) (exp_bound_uc z) _.
+  unary_complete_uc QPrelengthSpace coerce (λ x, AQexp (min ('z) x)) (exp_bound_uc z) _.
 Next Obligation. 
   intros. 
-  rewrite ARexp_correct, aq_preserves_min, AQtoQ_ZtoAQ.
+  rewrite AQexp_correct, aq_preserves_min, AQtoQ_ZtoAQ.
   reflexivity.
 Qed.
 
 Definition ARexp_bounded (z : Z) := Cbind AQPrelengthSpace (ARexp_bounded_uc z).
 
 Lemma ARtoCR_preserves_exp_bounded z x : ARtoCR (ARexp_bounded z x) = exp_bounded z (ARtoCR x).
-Proof. apply (preserves_unary_complete_fun QPrelengthSpace coerce (λ x, AQexp (min ('z : AQ) x))). Qed.
+Proof. apply (preserves_unary_complete_fun QPrelengthSpace coerce (λ x, AQexp (min ('z) x))). Qed.
 
 Definition ARexp (x : AR) : AR := ARexp_bounded (Qceiling ('approximate x (1#1)%Qpos + (1#1))) x.
 
